checkpoint: prototype propositional logic formation

LRA/VolumeI/PropositionalLogic/MetaLogic.lean
@@ -3,6 +3,7 @@ namespace LRA.VolumeI.PropositionalLogic
 -- 1. The Generic Signature
 structure Signature where
   Atoms : Type
+  UnaryOps : Type := Empty
   BinOps : Type := Empty
 
 -- 2. The Generic Language
@@ -10,17 +11,20 @@ inductive Formula (sig : Signature) where
   | atom : sig.Atoms → Formula sig
   | neg  : Formula sig → Formula sig
   | conj : Formula sig → Formula sig → Formula sig
+  | unary : sig.UnaryOps → Formula sig → Formula sig
   | binary : sig.BinOps → Formula sig → Formula sig → Formula sig
 
 -- 3. The Generic Semantics
 structure Structure (sig : Signature) where
   interpretation : sig.Atoms → Bool
+  evaluateUnary : sig.UnaryOps → Bool → Bool := fun _ _ => false
   evaluateBinary : sig.BinOps → Bool → Bool → Bool := fun _ _ _ => false
 
 def evaluate {sig : Signature} (M : Structure sig) : Formula sig → Bool
   | Formula.atom a   => M.interpretation a
   | Formula.neg ϕ    => !(evaluate M ϕ)
   | Formula.conj ϕ ψ => (evaluate M ϕ) && (evaluate M ψ)
+  | Formula.unary op ϕ => M.evaluateUnary op (evaluate M ϕ)
   | Formula.binary op ϕ ψ => M.evaluateBinary op (evaluate M ϕ) (evaluate M ψ)
 
 end LRA.VolumeI.PropositionalLogic
